StrictPositivity.v
@@ -1,0 +1,459 @@
+Require Import Equations.Equations.
+Require Import Equations.Subterm.
+
+Require Import Omega.
+
+Require Import Coq.Strings.String.
+Require Import Coq.Lists.List.
+
+Require Import Termination.StarInversions.
+Require Import Termination.StarRelation.
+Require Import Termination.SmallStep.
+Require Import Termination.Syntax.
+Require Import Termination.Trees.
+Require Import Termination.Tactics.
+Require Import Termination.Equivalence.
+Require Import Termination.OpenTOpen.
+
+Require Import Termination.SizeLemmas.
+
+Require Import Termination.WFLemmas.
+Require Import Termination.TWFLemmas.
+Require Import Termination.ErasedTermLemmas.
+
+Require Import Termination.ReducibilityCandidate.
+Require Import Termination.ReducibilityDefinition.
+Require Import Termination.ReducibilityLemmas.
+Require Import Termination.ReducibilityUnused.
+Require Import Termination.ReducibilityMeasure.
+Require Import Termination.ReducibilityRenaming.
+Require Import Termination.ReducibilitySubst.
+Require Import Termination.RedTactics.
+
+Require Import Termination.AssocList.
+Require Import Termination.Sets.
+Require Import Termination.Freshness.
+Require Import Termination.SwapHoles.
+Require Import Termination.ListUtils.
+Require Import Termination.TOpenTClose.
+
+Require Import Termination.FVLemmas.
+
+Opaque makeFresh.
+Opaque Nat.eq_dec.
+Opaque reducible_values.
+
+Fixpoint strictly_positive (t: tree) (k: nat) :=
+  match t with
+  | fvar _ type_var => True
+  | lvar i type_var => i <= k
+
+  | T_unit => True
+  | T_bool => True
+  | T_nat => True
+  | T_prod T1 T2 => strictly_positive T1 k /\ strictly_positive T2 k
+  | T_arrow T1 T2 => twf T1 k /\ strictly_positive T2 k
+  | T_sum T1 T2 => strictly_positive T1 k /\ strictly_positive T2 k
+  | T_refine T p => strictly_positive T k
+  | T_let t A B => strictly_positive B k
+  | T_singleton t => True
+  | T_intersection T1 T2 => strictly_positive T1 k /\ strictly_positive T2 k
+  | T_union T1 T2 => twf T1 k /\ twf T2 k (* !! TOOD: This could be relaxed by letting one hole in either T1 or T2 *)
+  | T_top => True
+  | T_bot => True
+  | T_equal t1 t2 => True
+  | T_forall T1 T2 => twf T1 k /\ strictly_positive T2 k
+  | T_exists T1 T2 => twf T1 k /\ twf T2 k (* !! We cannot push foralls down exists *)
+  | T_abs T => strictly_positive T (S k)
+  | T_rec n T0 Ts => strictly_positive T0 k /\ strictly_positive Ts (S k)
+
+  | _ => False
+  end.
+
+Lemma strictly_positive_open:
+  forall T k1 k2 rep,
+    twf rep 0 ->
+    strictly_positive T k1 ->
+    strictly_positive (open k2 T rep) k1.
+Proof.
+  induction T; steps; eauto using twf_open with btwf omega.
+Qed.
+
+Ltac t_topen_none :=
+  match goal with
+  | H1: twf ?T ?k, H2: context[topen ?k ?T ?rep] |- _ => rewrite (topen_none T k rep H1) in H2
+  | H1: twf ?T ?k |- context[topen ?k ?T ?rep] => rewrite (topen_none T k rep H1)
+  | H1: is_erased_term ?T, H2: context[topen ?k ?T ?rep] |- _ =>
+    rewrite (topen_none T k rep) in H2 by (steps; eauto with btwf)
+  | H1: is_erased_term ?T |- context[topen ?k ?T ?rep] =>
+    rewrite (topen_none T k rep) by (steps; eauto with btwf)
+  | H1: is_erased_term ?T, H2: context[topen ?k (open ?k' ?T ?rep') ?rep] |- _ =>
+    rewrite (topen_none (open k' T rep') k rep) in H2
+      by (repeat steps || apply twf_open; eauto 2 with btwf)
+  | H1: is_erased_term ?T |- context[topen ?k (open ?k' ?T ?rep') ?rep] =>
+    rewrite (topen_none (open k' T rep') k rep) by (repeat steps || apply twf_open; eauto 2 with btwf)
+  end.
+
+Ltac t_instantiate_reducible :=
+  match goal with
+  | H1: reducible_values _ ?v ?T, H2: is_erased_term ?v, H3: forall a, _ -> _ -> _ |- _ =>
+    poseNew (Mark (v,H3) "t_instantiate_reducible");
+    pose proof (H3 v H2 H1)
+  | H1: reducible_values _ ?v ?T, H2: forall a, _ -> _ |- _ =>
+    poseNew (Mark (v,H2) "t_instantiate_reducible");
+    pose proof (H2 v H1)
+  end.
+
+Ltac t_reduces_to :=
+  match goal with
+  | H: reduces_to ?P ?t |- reduces_to ?P' ?t => apply (reduces_to_equiv P P' t H)
+  end.
+
+Definition non_empty theta A := exists v, reducible_values theta v A.
+
+Lemma instantiate_non_empty:
+  forall theta (A: tree) (P: tree -> Prop),
+    non_empty theta A ->
+    (forall a, reducible_values theta a A -> P a) ->
+    exists a, reducible_values theta a A /\ P a.
+Proof.
+  unfold non_empty; steps; eauto.
+Qed.
+
+Ltac t_instantiate_non_empty :=
+  match goal with
+  | H1: non_empty ?theta ?A, H2: forall a, reducible_values ?theta a ?A -> _ |- _ =>
+    pose proof (instantiate_non_empty _ _ _ H1 H2)
+  end.
+
+Ltac apply_induction H :=
+  match goal with
+  | |- reducible_values _ _ (topen 0 ?T _) => apply H with (size T, index T)
+  end.
+
+Ltac find_smallstep_value :=
+  match goal with
+  | H: star small_step ?t ?v |- exists v, star small_step ?t v /\ _ => exists v
+  | H: star small_step ?t ?v |- exists x _, _ /\ _ /\ star small_step ?t x /\ _ => exists v
+  end.
+
+Ltac find_exists :=
+  match goal with
+  | |- exists a b _, pp ?c ?d = pp a b /\ _ => exists c, d
+  | |- (exists x, tleft ?v = tleft x /\ _) \/ _  => left; exists v
+  | |- _ \/ (exists x, tright ?v = tright x /\ _)  => right; exists v
+  end.
+
+Ltac find_reducible_value :=
+  match goal with
+  | H: reducible_values ?theta ?v (topen 0 ?T _) |-
+      exists a _, reducible_values ?theta a (topen 0 ?T _) /\ _ => exists v
+  end.
+
+Ltac reducibility_choice :=
+  match goal with
+  | H: reducible_values ?theta ?v (topen 0 ?T _) |-
+      reducible_values ?theta ?v (topen 0 ?T _) \/ _ => left
+  | H: reducible_values ?theta ?v (topen 0 ?T _) |-
+      _ \/ reducible_values ?theta ?v (topen 0 ?T _) => right
+  end.
+
+Lemma twf_positive:
+  forall T k,
+    is_erased_type T ->
+    twf T k ->
+    strictly_positive T k.
+Proof.
+  induction T; steps; try omega.
+Qed.
+
+Lemma swap_nothing:
+  forall T k i j,
+    twf T k ->
+    k <= i ->
+    k <= j ->
+    swap_type_holes T i j = T.
+Proof.
+  induction T; repeat step || tequality; eauto with omega.
+Qed.
+
+Lemma is_erased_swap:
+  forall T i j,
+    is_erased_type T ->
+    is_erased_type (swap_type_holes T i j).
+Proof.
+  induction T; repeat step || apply_any || rewrite (swap_nothing _ 0);
+    eauto with omega btwf.
+Qed.
+
+Hint Resolve is_erased_swap: berased.
+
+Lemma twf_swap:
+  forall T k rep,
+    twf rep 0 ->
+    twf T (S k) ->
+    twf (topen (S k) (swap_type_holes T k (S k)) rep) k.
+Proof.
+  induction T; steps; eauto with btwf omega.
+Qed.
+
+Hint Resolve twf_swap: btwf.
+
+Lemma twf_swap2:
+  forall T k rep,
+    twf rep 0 ->
+    twf T (S (S k)) ->
+    twf (topen (S k) (swap_type_holes T k (S k)) rep) (S k).
+Proof.
+  induction T; repeat step || unshelve eauto with btwf omega.
+Qed.
+
+Hint Resolve twf_swap2: btwf.
+
+Lemma wf_swap:
+  forall T k i j,
+    wf T k ->
+    wf (swap_type_holes T i j) k.
+Proof.
+  induction T; steps.
+Qed.
+
+Hint Resolve wf_swap: bwf.
+
+Ltac t_instantiate_rc :=
+  match goal with
+  | H: reducibility_candidate ?RC, H2: forall R, reducibility_candidate R -> _ |- _ =>
+     poseNew (Mark (H,H2) "instantiate_rc");
+     pose proof (H2 RC H)
+  end.
+
+Lemma strict_positive_monotone:
+  forall T k1 k2,
+    strictly_positive T k1 ->
+    k1 <= k2 ->
+    strictly_positive T k2.
+Proof.
+  induction T;
+    repeat step;
+    eauto with btwf omega.
+Qed.
+
+Lemma strictly_positive_swap:
+  forall T i rep,
+    twf rep 0 ->
+    is_erased_type T ->
+    strictly_positive rep 0 ->
+    strictly_positive T (S i) ->
+    strictly_positive (topen (S i) (swap_type_holes T i (S i)) rep) i.
+Proof.
+  induction T; repeat step || apply twf_swap;
+    eauto using strict_positive_monotone with omega.
+Qed.
+
+Lemma non_empty_extend:
+  forall theta A x RC,
+    non_empty theta A ->
+    reducibility_candidate RC ->
+    valid_interpretation theta ->
+    ~(x ∈ pfv A type_var) ->
+    non_empty ((x, RC) :: theta) A.
+Proof.
+  unfold non_empty; repeat step || exists v || apply reducible_unused2.
+Qed.
+
+Lemma valid_interpretation_cons:
+  forall theta RC X,
+    valid_interpretation theta ->
+    reducibility_candidate RC ->
+    valid_interpretation ((X, RC) :: theta).
+Proof.
+  steps.
+Qed.
+
+Lemma swap_holes_twice:
+  forall T i j,
+    swap_type_holes (swap_type_holes T i j) i j = T.
+Proof.
+  induction T; steps.
+Qed.
+
+Ltac t_reducible_rename_one :=
+  match goal with
+  | H: reducible_values ((?X,?RC) :: ?theta) ?v (topen 0 ?T (fvar ?X type_var)) |-
+       reducible_values ((?Y,?RC) :: ?theta) ?v (topen 0 ?T (fvar ?Y type_var)) =>
+    apply reducible_rename_one with X
+  end.
+
+Lemma fv_in_reducible_val:
+  forall theta v T x tag,
+    reducible_values theta v T ->
+    valid_interpretation theta ->
+    x ∈ pfv v tag ->
+    False.
+Proof.
+  intros. erewrite reducible_val_fv in *; eauto.
+Qed.
+
+Lemma strictly_positive_push_forall:
+  forall measure T theta A B v,
+    (size T, index T) = measure ->
+    strictly_positive T 0 ->
+    wf T 0 ->
+    twf T 1 ->
+    wf A 0 ->
+    twf A 0 ->
+    wf B 1 ->
+    twf B 0 ->
+    valid_interpretation theta ->
+    non_empty theta A ->
+    is_erased_type A ->
+    is_erased_type B ->
+    is_erased_type T ->
+    (forall a,
+      reducible_values theta a A ->
+      reducible_values theta v (topen 0 T (open 0 B a))) ->
+    reducible_values theta v (topen 0 T (T_forall A B)).
+Proof.
+  induction measure as [ PP HH ] using measure_induction; intros; t_instantiate_non_empty; destruct T;
+    repeat match goal with
+    | _ =>
+      step ||
+      simp_red ||
+      t_topen_none ||
+      t_instantiate_reducible ||
+      find_reducible_value ||
+      reducibility_choice ||
+      t_deterministic_star ||
+      (* t_reduces_to || *)
+      ( progress unfold reduces_to in * ) ||
+      find_smallstep_value ||
+      apply strictly_positive_open ||
+      apply left_lex ||
+      apply_induction HH ||
+      find_exists ||
+      ( progress autorewrite with bsize in * ) ||
+      (rewrite open_topen in * by (steps; eauto with btwf; eauto with bwf))
+    end;
+    try omega;
+    eauto using reducible_values_closed;
+    eauto with berased bwf btwf;
+    try solve [ apply twf_open; eauto with btwf ].
+
+  (** Polymorphic type **)
+  - exists (makeFresh (
+           support theta ::
+           pfv A type_var ::
+           pfv T type_var ::
+           pfv B type_var ::
+           pfv (topen 1 T (T_forall A B)) type_var :: nil));
+      repeat step || finisher || t_instantiate_rc || find_smallstep_value;
+        try solve [ repeat unfold closed_term, closed_value in * || step ].
+
+    rewrite open_swap; steps; eauto with omega.
+    apply_induction HH;
+      repeat
+        step ||
+        apply left_lex ||
+        (progress autorewrite with bsize in * ) ||
+        apply strictly_positive_swap ||
+        apply twf_topen ||
+        apply is_erased_type_topen ||
+        apply non_empty_extend ||
+        t_deterministic_star ||
+        apply wf_topen;
+      try finisher;
+      eauto with bwf btwf omega berased;
+      eauto 2 using red_is_val with step_tactic.
+
+    apply reducible_unused3 in H27; steps; try finisher.
+
+    rewrite open_swap;
+      repeat step || rewrite swap_holes_twice ||
+             t_instantiate_reducible || t_instantiate_rc ||
+             unfold reduces_to in * || t_deterministic_star ||
+             simp_red || t_reducible_rename_one || t_fv_open ||
+             t_listutils ||
+             unshelve eauto using valid_interpretation_cons with btwf btwf2 ||
+             unshelve eauto using valid_interpretation_cons, red_is_val;
+      try finisher;
+      eauto using fv_in_reducible_val.
+
+  (** Recursive type at 0 **)
+  - left.
+      repeat step || simp_red ||
+             t_instantiate_reducible || apply_induction HH || apply left_lex ||
+             t_deterministic_star ||
+             t_topen_none; eauto with omega.
+
+  (** Recursive type at n+1 **)
+  - right.
+      exists n'0, v'0, (makeFresh (
+                       support theta ::
+                       pfv A type_var ::
+                       pfv n'0 type_var ::
+                       pfv (topen 0 T2 (T_forall A B)) type_var ::
+                       pfv (topen 1 T3 (T_forall A B)) type_var ::
+                       nil));
+      repeat step || simp_red ||
+             t_instantiate_reducible || apply_induction HH || apply left_lex ||
+             t_deterministic_star ||
+             t_topen_none;
+        eauto with omega;
+        try finisher.
+
+      remember (makeFresh (
+                       support theta ::
+                       pfv A type_var ::
+                       pfv n'0 type_var ::
+                       pfv (topen 0 T2 (T_forall A B)) type_var ::
+                       pfv (topen 1 T3 (T_forall A B)) type_var ::
+                       nil)) as M.
+
+      apply reducibility_subst_head2;
+        repeat
+          step || t_listutils ||
+          apply is_erased_topen ||
+          apply is_erased_type_topen ||
+          apply twf_topen ||
+          apply wf_topen;
+        try finisher;
+        eauto with btwf;
+        eauto with bwf.
+
+     (*
+    topen 0 (topen 1 A R) (topen 0 B R)
+*)
+(*
+      rewrite open_swap;
+      repeat step || apply twf_topen;
+      eauto with omega;
+      eauto with btwf.
+*)
+    (*
+    assert (
+      topen 0 (topen 1 A (topen 0 B R)) R
+      topen 0 (t_close 0 (topen 1 A (topen 0 B X)) X) R
+    ).
+*)
+Admitted.
+
+Lemma strictly_positive_pull_forall:
+  forall T theta A B v a,
+    strictly_positive T 0 ->
+    wf T 0 ->
+    twf T 1 ->
+    wf A 0 ->
+    twf A 0 ->
+    wf B 1 ->
+    twf B 0 ->
+    valid_interpretation theta ->
+    reducible_values theta a A ->
+    reducible_values theta v (topen 0 T (T_forall A B)) ->
+    reducible_values theta v (topen 0 T (open 0 B a)).
+Proof.
+(*  induction T;
+    repeat t_topen_none || step ||
+      simp reducible_values in * ||
+      (rewrite topen_none in * by t_rewrite);
+    eauto 6 with berased; eauto 11. *)
+Admitted.
