TOpenTClose.v
@@ -1,0 +1,53 @@
+Require Import Coq.Strings.String.
+Require Import Omega.
+
+Require Import Termination.Syntax.
+Require Import Termination.Tactics.
+Require Import Termination.AssocList.
+Require Import Termination.Sets.
+Require Import Termination.ListUtils.
+Require Import Termination.TWFLemmas.
+Require Import Termination.SubstitutionLemmas.
+Require Import Termination.FVLemmas.
+
+Open Scope string_scope.
+Open Scope list_scope.
+
+Opaque Nat.eq_dec.
+
+Lemma topen_tclose:
+  forall T rep x k,
+    twf T k ->
+    topen k (tclose k T x) rep = psubstitute T ((x, rep) :: nil) type_var.
+Proof.
+  induction T;
+    repeat step || tequality || t_listutils; eauto with omega.
+Qed.
+
+(*
+  topen 0 (topen 1 A (topen 0 B R)) R =
+  topen k (tclose 0 (topen 1 A (topen 0 B X))) R
+*)
+
+Lemma topen_twice:
+  forall A B R X k,
+    ~(X ∈ pfv A type_var) ->
+    ~(X ∈ pfv B type_var) ->
+    twf A (S (S k)) ->
+    twf B 1 ->
+    twf R 0 ->
+      topen k (topen (S k) A (topen 0 B R)) R =
+      topen k (tclose k (topen (S k) A (topen 0 B (fvar X type_var))) X) R.
+Proof.
+  induction A; repeat step || tequality || apply_any || t_listutils;
+    eauto with btwf omega.
+  - rewrite topen_tclose;
+      repeat step || t_fv_open || t_listutils || apply twf_topen;
+      eauto with btwf omega.
+    + rewrite substitute_topen3; steps.
+      rewrite substitute_nothing; steps.
+      rewrite topen_none; steps; eauto with btwf.
+      apply twf_monotone with 0; eauto with btwf omega.
+    + apply twf_monotone with 0; try omega.
+      apply twf_topen; steps.
+Qed.
